Migrate correctness to PosTracker

correctness/RegexCorrectness/Backtracker/Refinement.lean
@@ -2,39 +2,41 @@ module
 
 import all RegexCorrectness.Backtracker.Traversal
 import all RegexCorrectness.Strategy.Materialize.Basic
+import all RegexCorrectness.Strategy.Materialize.Lemmas
 import RegexCorrectness.Strategy
+import Regex.Strategy
 
 open Regex (NFA)
 open Regex.Data (BitMatrix BVPos)
-open Regex.Strategy (materializeUpdates)
+open Regex.Strategy (materializeUpdates materializeUpdates_snoc)
 open String (Pos PosPlusOne)
 namespace Regex.Backtracker
 
 variable {s : String} {nfa : NFA} {wf : nfa.WellFormed} {startPos : Pos s} {bufferSize : Nat}
 
-def StackEntry.materialize (entryH : StackEntry (HistoryStrategy s) nfa startPos) : StackEntry (BufferStrategy s bufferSize) nfa startPos :=
+def StackEntry.materialize (entryH : StackEntry (List (Nat × Pos s)) nfa startPos) : StackEntry (Vector (PosPlusOne s) bufferSize) nfa startPos :=
   ⟨materializeUpdates bufferSize entryH.update, entryH.state, entryH.pos⟩
 
-def materializeStack (stackH : List (StackEntry (HistoryStrategy s) nfa startPos)) : List (StackEntry (BufferStrategy s bufferSize) nfa startPos) :=
+def materializeStack (stackH : List (StackEntry (List (Nat × Pos s)) nfa startPos)) : List (StackEntry (Vector (PosPlusOne s) bufferSize) nfa startPos) :=
   stackH.map StackEntry.materialize
 
 @[simp]
-theorem materializeStack.nil : materializeStack [] = ([] : List (StackEntry (BufferStrategy s bufferSize) nfa startPos)) := rfl
+theorem materializeStack.nil : materializeStack [] = ([] : List (StackEntry (Vector (PosPlusOne s) bufferSize) nfa startPos)) := rfl
 
 @[simp]
 theorem materializeStack.cons {entryH stackH} :
-  materializeStack (entryH :: stackH) = (StackEntry.materialize entryH :: materializeStack stackH : List (StackEntry (BufferStrategy s bufferSize) nfa startPos)) := rfl
+  materializeStack (entryH :: stackH) = (StackEntry.materialize entryH :: materializeStack stackH : List (StackEntry (Vector (PosPlusOne s) bufferSize) nfa startPos)) := rfl
 
-def materializeResultAux (resultH : Option (List (Nat × Pos s)) × BitMatrix nfa.size (startPos.remainingBytes + 1)) : Option (Buffer s bufferSize) × BitMatrix nfa.size (startPos.remainingBytes + 1) :=
+def materializeResultAux (resultH : Option (List (Nat × Pos s)) × BitMatrix nfa.size (startPos.remainingBytes + 1)) : Option (Vector (PosPlusOne s) bufferSize) × BitMatrix nfa.size (startPos.remainingBytes + 1) :=
   ⟨resultH.1.map (materializeUpdates bufferSize), resultH.2⟩
 
-def materializeResult (resultH : Option (List (Nat × Pos s))) : Option (Buffer s bufferSize) :=
+def materializeResult (resultH : Option (List (Nat × Pos s))) : Option (Vector (PosPlusOne s) bufferSize) :=
   resultH.map (materializeUpdates bufferSize)
 
 theorem captureNextAux.pushNext.refines {s nfa wf startPos bufferSize stackH stackB updateH updateB state pos}
   (refEntry : StackEntry.materialize ⟨updateH, state, pos⟩ = ⟨updateB, state, pos⟩) (refStack : materializeStack stackH = stackB) :
-  materializeStack (captureNextAux.pushNext (HistoryStrategy s) nfa wf startPos stackH updateH state pos) = captureNextAux.pushNext (BufferStrategy s bufferSize) nfa wf startPos stackB updateB state pos := by
-  cases stackH, updateH, state, pos using captureNextAux.pushNext.fun_cases' (HistoryStrategy s) nfa wf startPos with
+  materializeStack (captureNextAux.pushNext (listTracker s) nfa wf startPos stackH updateH state pos) = captureNextAux.pushNext (vectorTracker s bufferSize) nfa wf startPos stackB updateB state pos := by
+  cases stackH, updateH, state, pos using captureNextAux.pushNext.fun_cases' nfa wf startPos with
   | done stackH updateH state pos hn => simp [pushNext.done hn, refStack]
   | fail stackH updateH state pos hn => simp [pushNext.fail hn, refStack]
   | epsilon stackH updateH state pos state' hn =>
@@ -45,7 +47,7 @@ theorem captureNextAux.pushNext.refines {s nfa wf startPos bufferSize stackH sta
     simp [pushNext.split hn, StackEntry.materialize, refStack, refEntry]
   | save stackH updateH state pos offset state' hn =>
     simp [StackEntry.materialize] at refEntry
-    simp [pushNext.save hn, StackEntry.materialize, refStack, refEntry]
+    simp [pushNext.save hn, StackEntry.materialize, refStack, refEntry, listTracker, vectorTracker, materializeUpdates_snoc]
   | anchor_pos stackH updateH state pos a state' hn ht =>
     simp [StackEntry.materialize] at refEntry
     simp [pushNext.anchor_pos hn ht, StackEntry.materialize, refStack, refEntry]
@@ -63,8 +65,8 @@ theorem captureNextAux.pushNext.refines {s nfa wf startPos bufferSize stackH sta
     simp [pushNext.sparse_neg hn h, refStack]
 
 theorem captureNextAux.refines {s} (nfa wf startPos bufferSize visited) {stackH stackB} (refStack : materializeStack stackH = stackB) :
-  materializeResultAux (captureNextAux (HistoryStrategy s) nfa wf startPos visited stackH) = captureNextAux (BufferStrategy s bufferSize) nfa wf startPos visited stackB := by
-  induction visited, stackH using captureNextAux.induct' (HistoryStrategy s) nfa wf startPos generalizing stackB with
+  materializeResultAux (captureNextAux (listTracker s) nfa wf startPos visited stackH) = captureNextAux (vectorTracker s bufferSize) nfa wf startPos visited stackB := by
+  induction visited, stackH using captureNextAux.induct' (listTracker s) nfa wf startPos generalizing stackB with
   | base visited =>
     simp at refStack
     simp [refStack, captureNextAux_base, materializeResultAux]
@@ -80,23 +82,23 @@ theorem captureNextAux.refines {s} (nfa wf startPos bufferSize visited) {stackH 
     exact ih (pushNext.refines rfl rfl)
 
 theorem captureNext.go.refines {s} (nfa wf startPos bufferSize bvpos visited) :
-  materializeResult (captureNext.go (HistoryStrategy s) nfa wf startPos bvpos visited) = captureNext.go (BufferStrategy s bufferSize) nfa wf startPos bvpos visited := by
-  induction bvpos, visited using captureNext.go.induct' (HistoryStrategy s) nfa wf startPos with
+  materializeResult (captureNext.go (listTracker s) nfa wf startPos bvpos visited) = captureNext.go (vectorTracker s bufferSize) nfa wf startPos bvpos visited := by
+  induction bvpos, visited using captureNext.go.induct' (List (Nat × Pos s)) (listTracker s) nfa wf startPos with
   | found bvpos visited updateH visitedH hauxH =>
-    have hauxB := captureNextAux.refines nfa wf startPos bufferSize visited rfl (stackB := materializeStack [⟨(HistoryStrategy s).empty, ⟨nfa.start, wf.start_lt⟩, bvpos⟩])
+    have hauxB := captureNextAux.refines nfa wf startPos bufferSize visited rfl (stackB := materializeStack [⟨(listTracker s).empty, ⟨nfa.start, wf.start_lt⟩, bvpos⟩])
     simp [↓hauxH, materializeResultAux] at hauxB
     simp [captureNext.go_found hauxH, captureNext.go_found hauxB.symm, materializeResult]
   | not_found_next bvpos visited visitedH hauxH ne ih =>
-    have hauxB := captureNextAux.refines nfa wf startPos bufferSize visited rfl (stackB := materializeStack [⟨(HistoryStrategy s).empty, ⟨nfa.start, wf.start_lt⟩, bvpos⟩])
+    have hauxB := captureNextAux.refines nfa wf startPos bufferSize visited rfl (stackB := materializeStack [⟨(listTracker s).empty, ⟨nfa.start, wf.start_lt⟩, bvpos⟩])
     simp [↓hauxH, materializeResultAux] at hauxB
     simpa [captureNext.go_not_found_next hauxH ne, captureNext.go_not_found_next hauxB.symm ne] using ih
   | not_found_end bvpos visited visitedH hauxH ne =>
-    have hauxB := captureNextAux.refines nfa wf startPos bufferSize visited rfl (stackB := materializeStack [⟨(HistoryStrategy s).empty, ⟨nfa.start, wf.start_lt⟩, bvpos⟩])
+    have hauxB := captureNextAux.refines nfa wf startPos bufferSize visited rfl (stackB := materializeStack [⟨(listTracker s).empty, ⟨nfa.start, wf.start_lt⟩, bvpos⟩])
     simp [↓hauxH, materializeResultAux] at hauxB
     simp [captureNext.go_not_found_end hauxH ne, captureNext.go_not_found_end hauxB.symm ne, materializeResult]
 
 theorem captureNext.refines {s} (nfa wf bufferSize pos) :
-  materializeResult (captureNext (HistoryStrategy s) nfa wf pos) = captureNext (BufferStrategy s bufferSize) nfa wf pos := by
+  materializeResult (captureNext (listTracker s) nfa wf pos) = captureNext (vectorTracker s bufferSize) nfa wf pos := by
   simpa [captureNext] using captureNext.go.refines nfa wf pos bufferSize (BVPos.start pos) (BitMatrix.zero _ _)
 
 end Regex.Backtracker
