correctness/RegexCorrectness/Backtracker/Basic.lean
@@ -3,6 +3,7 @@ module
 import all Regex.Data.BitMatrix
 import all Regex.Data.BVPos
 import all Regex.Backtracker.Basic
+import Regex.Strategy
 import Mathlib.Tactic.DepRewrite
 
 open Regex.Data (BitMatrix BVPos)
@@ -12,59 +13,59 @@ namespace Regex.Backtracker
 
 namespace captureNextAux.pushNext
 
-variable {s : String} {σ : Strategy s} {nfa : NFA} {wf : nfa.WellFormed}
-  {startPos : Pos s} {stack : List (StackEntry σ nfa startPos)} {update : σ.Update} {state : Fin nfa.size} {pos : BVPos startPos}
+variable {s : String} {α : Type} {tracker : PosTracker s α} {nfa : NFA} {wf : nfa.WellFormed}
+  {startPos : Pos s} {stack : List (StackEntry α nfa startPos)} {update : α} {state : Fin nfa.size} {pos : BVPos startPos}
 
-theorem done (hn : nfa[state] = .done) : pushNext σ nfa wf startPos stack update state pos = stack := by
+theorem done (hn : nfa[state] = .done) : pushNext tracker nfa wf startPos stack update state pos = stack := by
   rw! [pushNext, hn]
   rfl
 
-theorem fail (hn : nfa[state] = .fail) : pushNext σ nfa wf startPos stack update state pos = stack := by
+theorem fail (hn : nfa[state] = .fail) : pushNext tracker nfa wf startPos stack update state pos = stack := by
   rw! [pushNext, hn]
   rfl
 
 theorem epsilon {state' : Nat} (hn : nfa[state] = .epsilon state') :
   haveI isLt : state' < nfa.size := wf.inBounds' state state.isLt hn
-  pushNext σ nfa wf startPos stack update state pos = ⟨update, ⟨state', isLt⟩, pos⟩ :: stack := by
+  pushNext tracker nfa wf startPos stack update state pos = ⟨update, ⟨state', isLt⟩, pos⟩ :: stack := by
   rw! [pushNext, hn]
   rfl
 
 theorem split {state₁ state₂ : Nat} (hn : nfa[state] = .split state₁ state₂) :
   haveI isLt : state₁ < nfa.size ∧ state₂ < nfa.size := wf.inBounds' state state.isLt hn
-  pushNext σ nfa wf startPos stack update state pos = ⟨update, ⟨state₁, isLt.1⟩, pos⟩ :: ⟨update, ⟨state₂, isLt.2⟩, pos⟩ :: stack := by
+  pushNext tracker nfa wf startPos stack update state pos = ⟨update, ⟨state₁, isLt.1⟩, pos⟩ :: ⟨update, ⟨state₂, isLt.2⟩, pos⟩ :: stack := by
   rw! [pushNext, hn]
   rfl
 
 theorem saveFin {offset : Nat} {state' : Fin nfa.size} (hn : nfa[state] = .save offset state') :
-  pushNext σ nfa wf startPos stack update state pos = ⟨σ.write update offset pos.current, state', pos⟩ :: stack := by
+  pushNext tracker nfa wf startPos stack update state pos = ⟨tracker.write update offset pos.current, state', pos⟩ :: stack := by
   rw! [pushNext, hn]
   rfl
 
 theorem save {offset state' : Nat} (hn : nfa[state] = .save offset state') :
   haveI isLt : state' < nfa.size := wf.inBounds' state state.isLt hn
-  pushNext σ nfa wf startPos stack update state pos = ⟨σ.write update offset pos.current, ⟨state', isLt⟩, pos⟩ :: stack := by
+  pushNext tracker nfa wf startPos stack update state pos = ⟨tracker.write update offset pos.current, ⟨state', isLt⟩, pos⟩ :: stack := by
   rw! [pushNext, hn]
   rfl
 
 theorem anchor_pos {a : Data.Anchor} {state' : Nat} (hn : nfa[state] = .anchor a state') (h : Data.Anchor.test pos.current a) :
   haveI isLt : state' < nfa.size := wf.inBounds' state state.isLt hn
-  pushNext σ nfa wf startPos stack update state pos = ⟨update, ⟨state', isLt⟩, pos⟩ :: stack := by
+  pushNext tracker nfa wf startPos stack update state pos = ⟨update, ⟨state', isLt⟩, pos⟩ :: stack := by
   rw! [pushNext, hn]
   simp [h]
 
 theorem anchor_neg {a : Data.Anchor} {state' : Nat} (hn : nfa[state] = .anchor a state') (h : ¬Data.Anchor.test pos.current a) :
-  pushNext σ nfa wf startPos stack update state pos = stack := by
+  pushNext tracker nfa wf startPos stack update state pos = stack := by
   rw! [pushNext, hn]
   simp [h]
 
 theorem char_pos {c : Char} {state' : Nat} (hn : nfa[state] = .char c state') (h : pos ≠ s.endBVPos startPos) (hc : pos.get h = c) :
   haveI isLt : state' < nfa.size := wf.inBounds' state state.isLt hn
-  pushNext σ nfa wf startPos stack update state pos = ⟨update, ⟨state', isLt⟩, pos.next h⟩ :: stack := by
+  pushNext tracker nfa wf startPos stack update state pos = ⟨update, ⟨state', isLt⟩, pos.next h⟩ :: stack := by
   rw! [pushNext, hn]
   simp [h, hc]
 
 theorem char_neg {c : Char} {state' : Nat} (hn : nfa[state] = .char c state') (h : pos = s.endBVPos startPos ∨ ∃ ne : pos ≠ s.endBVPos startPos, pos.get ne ≠ c) :
-  pushNext σ nfa wf startPos stack update state pos = stack := by
+  pushNext tracker nfa wf startPos stack update state pos = stack := by
   rw! [pushNext, hn]
   match h with
   | .inl h => simp [h]
@@ -72,42 +73,42 @@ theorem char_neg {c : Char} {state' : Nat} (hn : nfa[state] = .char c state') (h
 
 theorem sparse_pos {cs : Data.Classes} {state' : Nat} (hn : nfa[state] = .sparse cs state') (h : pos ≠ s.endBVPos startPos) (hc : pos.get h ∈ cs) :
   haveI isLt : state' < nfa.size := wf.inBounds' state state.isLt hn
-  pushNext σ nfa wf startPos stack update state pos = ⟨update, ⟨state', isLt⟩, pos.next h⟩ :: stack := by
+  pushNext tracker nfa wf startPos stack update state pos = ⟨update, ⟨state', isLt⟩, pos.next h⟩ :: stack := by
   rw! [pushNext, hn]
   simp [h, hc]
 
 theorem sparse_neg {cs : Data.Classes} {state' : Nat} (hn : nfa[state] = .sparse cs state') (h : pos = s.endBVPos startPos ∨ ∃ ne : pos ≠ s.endBVPos startPos, pos.get ne ∉ cs) :
-  pushNext σ nfa wf startPos stack update state pos = stack := by
+  pushNext tracker nfa wf startPos stack update state pos = stack := by
   rw! [pushNext, hn]
   match h with
   | .inl h => simp [h]
   | .inr ⟨ne, hc⟩ => simp [ne, hc]
 
-theorem fun_cases' (σ : Strategy s) (nfa : NFA) (wf : nfa.WellFormed) (startPos : Pos s)
-  {motive : List (StackEntry σ nfa startPos) → σ.Update → Fin nfa.size → BVPos startPos → Prop}
-  (done : ∀ (stack : List (StackEntry σ nfa startPos)) (update : σ.Update) (state : Fin nfa.size) (pos : BVPos startPos),
+theorem fun_cases' {α : Type} (nfa : NFA) (wf : nfa.WellFormed) (startPos : Pos s)
+  {motive : List (StackEntry α nfa startPos) → α → Fin nfa.size → BVPos startPos → Prop}
+  (done : ∀ (stack : List (StackEntry α nfa startPos)) (update : α) (state : Fin nfa.size) (pos : BVPos startPos),
     nfa[state] = .done → motive stack update state pos)
-  (fail : ∀ (stack : List (StackEntry σ nfa startPos)) (update : σ.Update) (state : Fin nfa.size) (pos : BVPos startPos),
+  (fail : ∀ (stack : List (StackEntry α nfa startPos)) (update : α) (state : Fin nfa.size) (pos : BVPos startPos),
     nfa[state] = .fail → motive stack update state pos)
-  (epsilon : ∀ (stack : List (StackEntry σ nfa startPos)) (update : σ.Update) (state : Fin nfa.size) (pos : BVPos startPos) (state' : Fin nfa.size),
+  (epsilon : ∀ (stack : List (StackEntry α nfa startPos)) (update : α) (state : Fin nfa.size) (pos : BVPos startPos) (state' : Fin nfa.size),
     nfa[state] = .epsilon state' → motive stack update state pos)
-  (split : ∀ (stack : List (StackEntry σ nfa startPos)) (update : σ.Update) (state : Fin nfa.size) (pos : BVPos startPos) (state₁ state₂ : Fin nfa.size),
+  (split : ∀ (stack : List (StackEntry α nfa startPos)) (update : α) (state : Fin nfa.size) (pos : BVPos startPos) (state₁ state₂ : Fin nfa.size),
     nfa[state] = .split state₁ state₂ → motive stack update state pos)
-  (save : ∀ (stack : List (StackEntry σ nfa startPos)) (update : σ.Update) (state : Fin nfa.size) (pos : BVPos startPos) (offset : Nat) (state' : Fin nfa.size),
+  (save : ∀ (stack : List (StackEntry α nfa startPos)) (update : α) (state : Fin nfa.size) (pos : BVPos startPos) (offset : Nat) (state' : Fin nfa.size),
     nfa[state] = .save offset state' → motive stack update state pos)
-  (anchor_pos : ∀ (stack : List (StackEntry σ nfa startPos)) (update : σ.Update) (state : Fin nfa.size) (pos : BVPos startPos) (a : Data.Anchor) (state' : Fin nfa.size),
+  (anchor_pos : ∀ (stack : List (StackEntry α nfa startPos)) (update : α) (state : Fin nfa.size) (pos : BVPos startPos) (a : Data.Anchor) (state' : Fin nfa.size),
     nfa[state] = .anchor a state' → a.test pos.current → motive stack update state pos)
-  (anchor_neg : ∀ (stack : List (StackEntry σ nfa startPos)) (update : σ.Update) (state : Fin nfa.size) (pos : BVPos startPos) (a : Data.Anchor) (state' : Fin nfa.size),
+  (anchor_neg : ∀ (stack : List (StackEntry α nfa startPos)) (update : α) (state : Fin nfa.size) (pos : BVPos startPos) (a : Data.Anchor) (state' : Fin nfa.size),
     nfa[state] = .anchor a state' → ¬a.test pos.current → motive stack update state pos)
-  (char_pos : ∀ (stack : List (StackEntry σ nfa startPos)) (update : σ.Update) (state : Fin nfa.size) (pos : BVPos startPos) (c : Char) (state' : Fin nfa.size),
+  (char_pos : ∀ (stack : List (StackEntry α nfa startPos)) (update : α) (state : Fin nfa.size) (pos : BVPos startPos) (c : Char) (state' : Fin nfa.size),
     nfa[state] = .char c state' → (h : pos ≠ s.endBVPos startPos) → pos.get h = c → motive stack update state pos)
-  (char_neg : ∀ (stack : List (StackEntry σ nfa startPos)) (update : σ.Update) (state : Fin nfa.size) (pos : BVPos startPos) (c : Char) (state' : Fin nfa.size),
+  (char_neg : ∀ (stack : List (StackEntry α nfa startPos)) (update : α) (state : Fin nfa.size) (pos : BVPos startPos) (c : Char) (state' : Fin nfa.size),
     nfa[state] = .char c state' → (pos = s.endBVPos startPos ∨ ∃ ne : pos ≠ s.endBVPos startPos, pos.get ne ≠ c) → motive stack update state pos)
-  (sparse_pos : ∀ (stack : List (StackEntry σ nfa startPos)) (update : σ.Update) (state : Fin nfa.size) (pos : BVPos startPos) (cs : Data.Classes) (state' : Fin nfa.size),
+  (sparse_pos : ∀ (stack : List (StackEntry α nfa startPos)) (update : α) (state : Fin nfa.size) (pos : BVPos startPos) (cs : Data.Classes) (state' : Fin nfa.size),
     nfa[state] = .sparse cs state' → (h : pos ≠ s.endBVPos startPos) → pos.get h ∈ cs → motive stack update state pos)
-  (sparse_neg : ∀ (stack : List (StackEntry σ nfa startPos)) (update : σ.Update) (state : Fin nfa.size) (pos : BVPos startPos) (cs : Data.Classes) (state' : Fin nfa.size),
+  (sparse_neg : ∀ (stack : List (StackEntry α nfa startPos)) (update : α) (state : Fin nfa.size) (pos : BVPos startPos) (cs : Data.Classes) (state' : Fin nfa.size),
     nfa[state] = .sparse cs state' → (pos = s.endBVPos startPos ∨ ∃ ne : pos ≠ s.endBVPos startPos, pos.get ne ∉ cs) → motive stack update state pos)
-  : ∀ (stack : List (StackEntry σ nfa startPos)) (update : σ.Update) (state : Fin nfa.size) (pos : BVPos startPos),
+  : ∀ (stack : List (StackEntry α nfa startPos)) (update : α) (state : Fin nfa.size) (pos : BVPos startPos),
     motive stack update state pos :=
   fun stack update state pos =>
     match hn : nfa[state] with
@@ -155,24 +156,24 @@ theorem fun_cases' (σ : Strategy s) (nfa : NFA) (wf : nfa.WellFormed) (startPos
 
 end captureNextAux.pushNext
 
-theorem captureNextAux.induct' {s : String} (σ : Strategy s) (nfa : NFA) (wf : nfa.WellFormed) (startPos : Pos s)
-  (motive : BitMatrix nfa.size (startPos.remainingBytes + 1) → List (StackEntry σ nfa startPos) → Prop)
+theorem captureNextAux.induct' {s : String} {α : Type} (tracker : PosTracker s α) (nfa : NFA) (wf : nfa.WellFormed) (startPos : Pos s)
+  (motive : BitMatrix nfa.size (startPos.remainingBytes + 1) → List (StackEntry α nfa startPos) → Prop)
   (base : ∀ (visited : BitMatrix nfa.size (startPos.remainingBytes + 1)), motive visited [])
-  (visited : ∀ (visited : BitMatrix nfa.size (startPos.remainingBytes + 1)) (update : σ.Update) (state : Fin nfa.size) (pos : BVPos startPos) (stack' : List (StackEntry σ nfa startPos)),
+  (visited : ∀ (visited : BitMatrix nfa.size (startPos.remainingBytes + 1)) (update : α) (state : Fin nfa.size) (pos : BVPos startPos) (stack' : List (StackEntry α nfa startPos)),
     visited.get state pos.index →
     motive visited stack' →
     motive visited (⟨update, state, pos⟩ :: stack'))
-  (done : ∀ (visited : BitMatrix nfa.size (startPos.remainingBytes + 1)) (update : σ.Update) (state : Fin nfa.size) (pos : BVPos startPos) (stack' : List (StackEntry σ nfa startPos)),
+  (done : ∀ (visited : BitMatrix nfa.size (startPos.remainingBytes + 1)) (update : α) (state : Fin nfa.size) (pos : BVPos startPos) (stack' : List (StackEntry α nfa startPos)),
     ¬visited.get state pos.index →
     nfa[state] = .done →
     motive visited (⟨update, state, pos⟩ :: stack'))
-  (next : ∀ (visited : BitMatrix nfa.size (startPos.remainingBytes + 1)) (update : σ.Update) (state : Fin nfa.size) (pos : BVPos startPos) (stack' : List (StackEntry σ nfa startPos)),
+  (next : ∀ (visited : BitMatrix nfa.size (startPos.remainingBytes + 1)) (update : α) (state : Fin nfa.size) (pos : BVPos startPos) (stack' : List (StackEntry α nfa startPos)),
     ¬visited.get state pos.index →
     nfa[state] ≠ .done →
-    motive (visited.set state pos.index) (pushNext σ nfa wf startPos stack' update state pos) →
+    motive (visited.set state pos.index) (pushNext tracker nfa wf startPos stack' update state pos) →
     motive visited (⟨update, state, pos⟩ :: stack'))
-  : ∀ (visited : BitMatrix nfa.size (startPos.remainingBytes + 1)) (stack : List (StackEntry σ nfa startPos)), motive visited stack :=
-  captureNextAux.induct σ nfa wf startPos motive
+  : ∀ (visited : BitMatrix nfa.size (startPos.remainingBytes + 1)) (stack : List (StackEntry α nfa startPos)), motive visited stack :=
+  captureNextAux.induct tracker nfa wf startPos motive
     base
     visited
     (fun visited update state bvpos stack' hmem _ hn => done visited update state bvpos stack' hmem (by simpa using hn))
@@ -183,21 +184,21 @@ Simplification lemmas for `captureNextAux`.
 -/
 section
 
-variable {s : String} {σ : Strategy s} {nfa : NFA} {wf : nfa.WellFormed} {startPos : Pos s} {visited : BitMatrix nfa.size (startPos.remainingBytes + 1)}
+variable {s : String} {α : Type} {tracker : PosTracker s α} {nfa : NFA} {wf : nfa.WellFormed} {startPos : Pos s} {visited : BitMatrix nfa.size (startPos.remainingBytes + 1)}
 
 theorem captureNextAux_base :
-  captureNextAux σ nfa wf startPos visited [] = (.none, visited) := by
+  captureNextAux tracker nfa wf startPos visited [] = (.none, visited) := by
   simp [captureNextAux]
 
 theorem captureNextAux_visited {update state pos stack'} (mem : visited.get state pos.index) :
-  captureNextAux σ nfa wf startPos visited (⟨update, state, pos⟩ :: stack') = captureNextAux σ nfa wf startPos visited stack' := by
+  captureNextAux tracker nfa wf startPos visited (⟨update, state, pos⟩ :: stack') = captureNextAux tracker nfa wf startPos visited stack' := by
   conv =>
     lhs
     unfold captureNextAux
     simp [mem]
 
 theorem captureNextAux_done {update state pos stack'} (mem : ¬visited.get state pos.index) (hn : nfa[state] = .done) :
-  captureNextAux σ nfa wf startPos visited (⟨update, state, pos⟩ :: stack') = (.some update, visited.set state pos.index) := by
+  captureNextAux tracker nfa wf startPos visited (⟨update, state, pos⟩ :: stack') = (.some update, visited.set state pos.index) := by
   simp at hn
   conv =>
     lhs
@@ -205,7 +206,7 @@ theorem captureNextAux_done {update state pos stack'} (mem : ¬visited.get state
     simp [mem, hn]
 
 theorem captureNextAux_next {update state pos stack'} (mem : ¬visited.get state pos.index) (hn : nfa[state] ≠ .done) :
-  captureNextAux σ nfa wf startPos visited (⟨update, state, pos⟩ :: stack') = captureNextAux σ nfa wf startPos (visited.set state pos.index) (captureNextAux.pushNext σ nfa wf startPos stack' update state pos) := by
+  captureNextAux tracker nfa wf startPos visited (⟨update, state, pos⟩ :: stack') = captureNextAux tracker nfa wf startPos (visited.set state pos.index) (captureNextAux.pushNext tracker nfa wf startPos stack' update state pos) := by
   simp at hn
   conv =>
     lhs
@@ -214,23 +215,23 @@ theorem captureNextAux_next {update state pos stack'} (mem : ¬visited.get state
 
 end
 
-theorem captureNext.go.induct' {s : String} (σ : Strategy s) (nfa : NFA) (wf : nfa.WellFormed) (startPos : Pos s)
+theorem captureNext.go.induct' {s : String} (α : Type) (tracker : PosTracker s α) (nfa : NFA) (wf : nfa.WellFormed) (startPos : Pos s)
   (motive : (pos : BVPos startPos) → BitMatrix nfa.size (startPos.remainingBytes + 1) → Prop)
-  (found : ∀ (pos : BVPos startPos) (visited : BitMatrix nfa.size (startPos.remainingBytes + 1)) (update : σ.Update) (visited' : BitMatrix nfa.size (startPos.remainingBytes + 1)),
-    captureNextAux σ nfa wf startPos visited [⟨σ.empty, ⟨nfa.start, wf.start_lt⟩, pos⟩] = (.some update, visited') →
+  (found : ∀ (pos : BVPos startPos) (visited : BitMatrix nfa.size (startPos.remainingBytes + 1)) (update : α) (visited' : BitMatrix nfa.size (startPos.remainingBytes + 1)),
+    captureNextAux tracker nfa wf startPos visited [⟨tracker.empty, ⟨nfa.start, wf.start_lt⟩, pos⟩] = (.some update, visited') →
     motive pos visited)
   (not_found_next : ∀ (pos : BVPos startPos) (visited visited' : BitMatrix nfa.size (startPos.remainingBytes + 1)),
-    captureNextAux σ nfa wf startPos visited [⟨σ.empty, ⟨nfa.start, wf.start_lt⟩, pos⟩] = (.none, visited') →
+    captureNextAux tracker nfa wf startPos visited [⟨tracker.empty, ⟨nfa.start, wf.start_lt⟩, pos⟩] = (.none, visited') →
     (h : pos ≠ s.endBVPos startPos) →
     (ih : motive (pos.next h) visited') →
     motive pos visited)
   (not_found_end : ∀ (pos : BVPos startPos) (visited visited' : BitMatrix nfa.size (startPos.remainingBytes + 1)),
-    captureNextAux σ nfa wf startPos visited [⟨σ.empty, ⟨nfa.start, wf.start_lt⟩, pos⟩] = (.none, visited') →
+    captureNextAux tracker nfa wf startPos visited [⟨tracker.empty, ⟨nfa.start, wf.start_lt⟩, pos⟩] = (.none, visited') →
     ¬pos ≠ s.endBVPos startPos →
     motive pos visited)
   (pos : BVPos startPos) (visited : BitMatrix nfa.size (startPos.remainingBytes + 1)) :
   motive pos visited :=
-  captureNext.go.induct σ nfa wf startPos motive
+  captureNext.go.induct tracker nfa wf startPos motive
     found not_found_next not_found_end pos visited
 
 /-
@@ -238,20 +239,20 @@ Simplification lemmas for `captureNext.go`.
 -/
 section
 
-variable {s : String} {σ : Strategy s} {nfa : NFA} {wf : nfa.WellFormed}
+variable {s : String} {α : Type} {tracker : PosTracker s α} {nfa : NFA} {wf : nfa.WellFormed}
   {startPos : Pos s} {visited : BitMatrix nfa.size (startPos.remainingBytes + 1)} {pos : BVPos startPos}
 
-theorem captureNext.go_found {update visited'} (h : captureNextAux σ nfa wf startPos visited [⟨σ.empty, ⟨nfa.start, wf.start_lt⟩, pos⟩] = (.some update, visited')) :
-  captureNext.go σ nfa wf startPos pos visited = .some update := by
+theorem captureNext.go_found {update visited'} (h : captureNextAux tracker nfa wf startPos visited [⟨tracker.empty, ⟨nfa.start, wf.start_lt⟩, pos⟩] = (.some update, visited')) :
+  captureNext.go tracker nfa wf startPos pos visited = .some update := by
   rw [captureNext.go, h]
 
-theorem captureNext.go_not_found_next {visited'} (h : captureNextAux σ nfa wf startPos visited [⟨σ.empty, ⟨nfa.start, wf.start_lt⟩, pos⟩] = (.none, visited')) (h' : pos ≠ s.endBVPos startPos) :
-  captureNext.go σ nfa wf startPos pos visited = captureNext.go σ nfa wf startPos (pos.next h') visited' := by
+theorem captureNext.go_not_found_next {visited'} (h : captureNextAux tracker nfa wf startPos visited [⟨tracker.empty, ⟨nfa.start, wf.start_lt⟩, pos⟩] = (.none, visited')) (h' : pos ≠ s.endBVPos startPos) :
+  captureNext.go tracker nfa wf startPos pos visited = captureNext.go tracker nfa wf startPos (pos.next h') visited' := by
   rw [captureNext.go, h]
   simp [h']
 
-theorem captureNext.go_not_found_end {visited'} (h : captureNextAux σ nfa wf startPos visited [⟨σ.empty, ⟨nfa.start, wf.start_lt⟩, pos⟩] = (.none, visited')) (h' : ¬pos ≠ s.endBVPos startPos) :
-  captureNext.go σ nfa wf startPos pos visited = .none := by
+theorem captureNext.go_not_found_end {visited'} (h : captureNextAux tracker nfa wf startPos visited [⟨tracker.empty, ⟨nfa.start, wf.start_lt⟩, pos⟩] = (.none, visited')) (h' : ¬pos ≠ s.endBVPos startPos) :
+  captureNext.go tracker nfa wf startPos pos visited = .none := by
   rw [captureNext.go, h]
   simp [h']
 
