correctness/RegexCorrectness/VM/CharStep/Basic.lean
@@ -1,6 +1,7 @@
 module
 
 import all RegexCorrectness.VM.EpsilonClosure
+import Regex.Strategy
 
 open Regex.Data (SparseSet)
 open Regex (NFA)
@@ -9,20 +10,20 @@ open String (Pos)
 namespace Regex.VM
 
 set_option linter.unusedVariables false in
-theorem eachStepChar.go.induct' {s : String} (σ : Strategy s) (nfa : NFA) (wf : nfa.WellFormed) (pos : Pos s) (ne : pos ≠ s.endPos) (current : SearchState σ nfa)
-  (motive : (i : Nat) → i ≤ current.states.count → SearchState σ nfa → Prop)
+theorem eachStepChar.go.induct' {s : String} (α : Type) (tracker : PosTracker s α) (nfa : NFA) (wf : nfa.WellFormed) (pos : Pos s) (ne : pos ≠ s.endPos) (current : SearchState α nfa)
+  (motive : (i : Nat) → i ≤ current.states.count → SearchState α nfa → Prop)
   (base : ∀ next, motive current.states.count (Nat.le_refl _) next)
   (done : ∀ i hlt next (hn : nfa[current.states[i]] = .done), motive i (Nat.le_of_lt hlt) next)
   (found : ∀ i hlt next (hn : nfa[current.states[i]] ≠ .done) matched next',
-    stepChar σ nfa wf pos ne current.updates next current.states[i] = (matched, next') →
+    stepChar tracker nfa wf pos ne current.updates next current.states[i] = (matched, next') →
     matched.isSome → motive i (Nat.le_of_lt hlt) next)
   (not_found : ∀ i hlt next (hn : nfa[current.states[i]] ≠ .done) matched next',
-    stepChar σ nfa wf pos ne current.updates next current.states[i] = (matched, next') →
+    stepChar tracker nfa wf pos ne current.updates next current.states[i] = (matched, next') →
     ¬matched.isSome → motive (i + 1) (by omega) next' →
     motive i (Nat.le_of_lt hlt) next)
-  (i : Nat) (hle : i ≤ current.states.count) (next : SearchState σ nfa) :
+  (i : Nat) (hle : i ≤ current.states.count) (next : SearchState α nfa) :
   motive i hle next := by
-  refine eachStepChar.go.induct σ nfa wf pos ne current motive ?base ?done ?found ?not_found i hle next
+  refine eachStepChar.go.induct tracker nfa wf pos ne current motive ?base ?done ?found ?not_found i hle next
   case base =>
     intro next _
     exact base next
@@ -37,31 +38,31 @@ theorem eachStepChar.go.induct' {s : String} (σ : Strategy s) (nfa : NFA) (wf :
     exact not_found i hlt next (by simpa using hn) result.1 result.2 rfl (by simp [notSome]) ih
 
 @[simp, grind =]
-theorem eachStepChar.go_base {s : String} {σ : Strategy s} {nfa wf pos ne current next} :
-  eachStepChar.go σ nfa wf pos ne current current.states.count (Nat.le_refl _) next = (.none, next) := by
+theorem eachStepChar.go_base {s : String} {α : Type} {tracker : PosTracker s α} {nfa wf pos ne current next} :
+  eachStepChar.go tracker nfa wf pos ne current current.states.count (Nat.le_refl _) next = (.none, next) := by
   grind [eachStepChar.go]
 
 @[simp, grind =]
-theorem eachStepChar.go_done {s : String} {σ : Strategy s} {nfa wf pos ne current i next}
+theorem eachStepChar.go_done {s : String} {α : Type} {tracker : PosTracker s α} {nfa wf pos ne current i next}
   (hlt : i < current.states.count)
   (hn : nfa[current.states[i]] = .done) :
-  eachStepChar.go σ nfa wf pos ne current i (Nat.le_of_lt hlt) next = (.none, next) := by
+  eachStepChar.go tracker nfa wf pos ne current i (Nat.le_of_lt hlt) next = (.none, next) := by
   grind [eachStepChar.go]
 
 @[simp, grind →]
-theorem eachStepChar.go_found {s : String} {σ : Strategy s} {nfa wf pos ne current i next next' matched}
+theorem eachStepChar.go_found {s : String} {α : Type} {tracker : PosTracker s α} {nfa wf pos ne current i next next' matched}
   (hlt : i < current.states.count)
   (hn : nfa[current.states[i]] ≠ .done)
-  (h : stepChar σ nfa wf pos ne current.updates next current.states[i] = (matched, next')) (found : matched.isSome) :
-  eachStepChar.go σ nfa wf pos ne current i (Nat.le_of_lt hlt) next = (matched, next') := by
+  (h : stepChar tracker nfa wf pos ne current.updates next current.states[i] = (matched, next')) (found : matched.isSome) :
+  eachStepChar.go tracker nfa wf pos ne current i (Nat.le_of_lt hlt) next = (matched, next') := by
   grind [eachStepChar.go]
 
 @[simp, grind →]
-theorem eachStepChar.go_not_found {s : String} {σ : Strategy s} {nfa wf pos ne current i next next' matched}
+theorem eachStepChar.go_not_found {s : String} {α : Type} {tracker : PosTracker s α} {nfa wf pos ne current i next next' matched}
   (hlt : i < current.states.count)
   (hn : nfa[current.states[i]] ≠ .done)
-  (h : stepChar σ nfa wf pos ne current.updates next current.states[i] = (matched, next')) (not_found : ¬matched.isSome) :
-  eachStepChar.go σ nfa wf pos ne current i (Nat.le_of_lt hlt) next = eachStepChar.go σ nfa wf pos ne current (i + 1) (by omega) next' := by
+  (h : stepChar tracker nfa wf pos ne current.updates next current.states[i] = (matched, next')) (not_found : ¬matched.isSome) :
+  eachStepChar.go tracker nfa wf pos ne current i (Nat.le_of_lt hlt) next = eachStepChar.go tracker nfa wf pos ne current (i + 1) (by omega) next' := by
   grind [eachStepChar.go]
 
 end Regex.VM
