correctness/RegexCorrectness/VM/EpsilonClosure/Basic.lean
@@ -3,6 +3,7 @@ module
 import all Regex.Data.SparseSet
 import all Regex.NFA.Basic
 import all Regex.VM
+import Regex.Strategy
 import all RegexCorrectness.VM.Path
 import Mathlib.Tactic.DepRewrite
 
@@ -17,78 +18,78 @@ namespace pushNext
 
 section
 
-variable {s : String} {σ : Strategy s} {nfa : NFA} {pos : Pos s} {node : Node} {inBounds : node.inBounds nfa.size} {update : σ.Update} {stack : εStack σ nfa}
+variable {s : String} {α : Type} {tracker : PosTracker s α} {nfa : NFA} {pos : Pos s} {node : Node} {inBounds : node.inBounds nfa.size} {update : α} {stack : εStack α nfa}
 
 @[grind =>]
 theorem epsilon {state' : Nat} (hn : node = .epsilon state') :
-  pushNext σ nfa pos node inBounds update stack = (update, ⟨state', by simp_all [Node.inBounds]⟩) :: stack := by
+  pushNext tracker nfa pos node inBounds update stack = (update, ⟨state', by simp_all [Node.inBounds]⟩) :: stack := by
   grind [pushNext]
 
 @[grind =>]
 theorem split {state₁ state₂ : Nat} (hn : node = .split state₁ state₂) :
-  pushNext σ nfa pos node inBounds update stack = (update, ⟨state₁, by simp_all [Node.inBounds]⟩) :: (update, ⟨state₂, by simp_all [Node.inBounds]⟩) :: stack := by
+  pushNext tracker nfa pos node inBounds update stack = (update, ⟨state₁, by simp_all [Node.inBounds]⟩) :: (update, ⟨state₂, by simp_all [Node.inBounds]⟩) :: stack := by
   grind [pushNext]
 
 @[grind =>]
 theorem save {offset state' : Nat} (hn : node = .save offset state') :
-  pushNext σ nfa pos node inBounds update stack = (σ.write update offset pos, ⟨state', by simp_all [Node.inBounds]⟩) :: stack := by
+  pushNext tracker nfa pos node inBounds update stack = (tracker.write update offset pos, ⟨state', by simp_all [Node.inBounds]⟩) :: stack := by
   grind [pushNext]
 
 @[grind =>]
 theorem anchor_pos {a : Anchor} {state' : Nat} (hn : node = .anchor a state') (ht : a.test pos) :
-  pushNext σ nfa pos node inBounds update stack = (update, ⟨state', by simp_all [Node.inBounds]⟩) :: stack := by
+  pushNext tracker nfa pos node inBounds update stack = (update, ⟨state', by simp_all [Node.inBounds]⟩) :: stack := by
   grind [pushNext]
 
 @[grind =>]
 theorem anchor_neg {a : Anchor} {state' : Nat} (hn : node = .anchor a state') (ht : ¬a.test pos) :
-  pushNext σ nfa pos node inBounds update stack = stack := by
+  pushNext tracker nfa pos node inBounds update stack = stack := by
   grind [pushNext]
 
 @[grind =>]
 theorem done (hn : node = .done) :
-  pushNext σ nfa pos node inBounds update stack = stack := by
+  pushNext tracker nfa pos node inBounds update stack = stack := by
   grind [pushNext]
 
 @[grind =>]
 theorem fail (hn : node = .fail) :
-  pushNext σ nfa pos node inBounds update stack = stack := by
+  pushNext tracker nfa pos node inBounds update stack = stack := by
   grind [pushNext]
 
 @[grind =>]
 theorem char {c : Char} {state' : Nat} (hn : node = .char c state') :
-  pushNext σ nfa pos node inBounds update stack = stack := by
+  pushNext tracker nfa pos node inBounds update stack = stack := by
   grind [pushNext]
 
 @[grind =>]
 theorem sparse {cs : Classes} {state' : Nat} (hn : node = .sparse cs state') :
-  pushNext σ nfa pos node inBounds update stack = stack := by
+  pushNext tracker nfa pos node inBounds update stack = stack := by
   grind [pushNext]
 
 end
 
-theorem fun_cases' {s : String} (σ : Strategy s) (nfa : NFA) (pos : Pos s)
-  {motive : (node : Node) → node.inBounds nfa.size → σ.Update → εStack σ nfa → Prop}
-  (epsilon : ∀ (update : σ.Update) (stack : εStack σ nfa) (state' : Nat) (inBounds : (Node.epsilon state').inBounds nfa.size),
+theorem fun_cases' {s : String} {α : Type} (nfa : NFA) (pos : Pos s)
+  {motive : (node : Node) → node.inBounds nfa.size → α → εStack α nfa → Prop}
+  (epsilon : ∀ (update : α) (stack : εStack α nfa) (state' : Nat) (inBounds : (Node.epsilon state').inBounds nfa.size),
     motive (Node.epsilon state') inBounds update stack)
-  (split : ∀ (update : σ.Update) (stack : εStack σ nfa) (state₁ state₂ : Nat) (inBounds : (Node.split state₁ state₂).inBounds nfa.size),
+  (split : ∀ (update : α) (stack : εStack α nfa) (state₁ state₂ : Nat) (inBounds : (Node.split state₁ state₂).inBounds nfa.size),
     motive (Node.split state₁ state₂) inBounds update stack)
-  (save : ∀ (update : σ.Update) (stack : εStack σ nfa) (offset state' : Nat) (inBounds : (Node.save offset state').inBounds nfa.size),
+  (save : ∀ (update : α) (stack : εStack α nfa) (offset state' : Nat) (inBounds : (Node.save offset state').inBounds nfa.size),
     motive (Node.save offset state') inBounds update stack)
-  (anchor_pos : ∀ (update : σ.Update) (stack : εStack σ nfa) (a : Anchor) (state' : Nat) (inBounds : (Node.anchor a state').inBounds nfa.size),
+  (anchor_pos : ∀ (update : α) (stack : εStack α nfa) (a : Anchor) (state' : Nat) (inBounds : (Node.anchor a state').inBounds nfa.size),
     a.test pos →
     motive (Node.anchor a state') inBounds update stack)
-  (anchor_neg : ∀ (update : σ.Update) (stack : εStack σ nfa) (a : Anchor) (state' : Nat) (inBounds : (Node.anchor a state').inBounds nfa.size),
+  (anchor_neg : ∀ (update : α) (stack : εStack α nfa) (a : Anchor) (state' : Nat) (inBounds : (Node.anchor a state').inBounds nfa.size),
     ¬a.test pos →
     motive (Node.anchor a state') inBounds update stack)
-  (done : ∀ (update : σ.Update) (stack : εStack σ nfa) (inBounds : Node.done.inBounds nfa.size),
+  (done : ∀ (update : α) (stack : εStack α nfa) (inBounds : Node.done.inBounds nfa.size),
     motive Node.done inBounds update stack)
-  (fail : ∀ (update : σ.Update) (stack : εStack σ nfa) (inBounds : Node.fail.inBounds nfa.size),
+  (fail : ∀ (update : α) (stack : εStack α nfa) (inBounds : Node.fail.inBounds nfa.size),
     motive Node.fail inBounds update stack)
-  (char : ∀ (update : σ.Update) (stack : εStack σ nfa) (c : Char) (state' : Nat) (inBounds : (Node.char c state').inBounds nfa.size),
+  (char : ∀ (update : α) (stack : εStack α nfa) (c : Char) (state' : Nat) (inBounds : (Node.char c state').inBounds nfa.size),
     motive (Node.char c state') inBounds update stack)
-  (sparse : ∀ (update : σ.Update) (stack : εStack σ nfa) (cs : Classes) (state' : Nat) (inBounds : (Node.sparse cs state').inBounds nfa.size),
+  (sparse : ∀ (update : α) (stack : εStack α nfa) (cs : Classes) (state' : Nat) (inBounds : (Node.sparse cs state').inBounds nfa.size),
     motive (Node.sparse cs state') inBounds update stack) :
-  ∀ (node : Node) (inBounds : node.inBounds nfa.size) (update : σ.Update) (stack : εStack σ nfa),
+  ∀ (node : Node) (inBounds : node.inBounds nfa.size) (update : α) (stack : εStack α nfa),
     motive node inBounds update stack :=
   fun node inBounds update stack =>
     match node with
@@ -110,24 +111,24 @@ end pushNext
 -- Cleaner version of the fuction induction principle
 -- It's crucial to annotate the types of the arguments of the branches. Otherwise, Lean consumse
 -- too much memory. See https://github.com/leanprover/lean4/issues/6753.
-theorem induct' {s : String} (σ : Strategy s) (nfa : NFA) (wf : nfa.WellFormed) (pos : Pos s)
-  (motive : Option σ.Update → SearchState σ nfa → εStack σ nfa → Prop)
-  (base : ∀ (matched : Option σ.Update) (next : SearchState σ nfa), motive matched next [])
-  (visited : ∀ (matched : Option σ.Update) (next : SearchState σ nfa) (update : σ.Update) (state : Fin nfa.size) (stack' : εStack σ nfa),
+theorem induct' {s : String} {α : Type} (tracker : PosTracker s α) (nfa : NFA) (wf : nfa.WellFormed) (pos : Pos s)
+  (motive : Option α → SearchState α nfa → εStack α nfa → Prop)
+  (base : ∀ (matched : Option α) (next : SearchState α nfa), motive matched next [])
+  (visited : ∀ (matched : Option α) (next : SearchState α nfa) (update : α) (state : Fin nfa.size) (stack' : εStack α nfa),
     state ∈ next.states →
     motive matched next stack' →
     motive matched next ((update, state) :: stack'))
-  (not_visited : ∀ (matched : Option σ.Update) (next : SearchState σ nfa) (update : σ.Update) (state : Fin nfa.size) (stack' : εStack σ nfa)
+  (not_visited : ∀ (matched : Option α) (next : SearchState α nfa) (update : α) (state : Fin nfa.size) (stack' : εStack α nfa)
     (hmem : state ∉ next.states),
     let node := nfa[state]
     let matched' := if node = Node.done then matched <|> some update else matched
     let states' := next.states.insert state hmem
     let updates' := if writeUpdate node = true then next.updates.set state update else next.updates
-    motive matched' ⟨states', updates'⟩ (pushNext σ nfa pos node (wf.inBounds state state.isLt) update stack') →
+    motive matched' ⟨states', updates'⟩ (pushNext tracker nfa pos node (wf.inBounds state state.isLt) update stack') →
     motive matched next ((update, state) :: stack')) :
-  ∀ (matched : Option σ.Update) (next : SearchState σ nfa) (stack : εStack σ nfa), motive matched next stack :=
+  ∀ (matched : Option α) (next : SearchState α nfa) (stack : εStack α nfa), motive matched next stack :=
   fun matched next stack =>
-    induct σ nfa wf pos motive base visited
+    induct tracker nfa wf pos motive base visited
       (fun matched update state stack' states updates hmem _ ih => by
         simp only [Node.isDone_def, decide_eq_true_eq] at ih
         exact not_visited matched ⟨states, updates⟩ update state stack' hmem ih)
@@ -138,14 +139,14 @@ Simplification lemmas for `εClosure`.
 -/
 section
 
-variable {s : String} {σ : Strategy s} {nfa : NFA} {wf : nfa.WellFormed} {pos : Pos s}
-  {matched : Option σ.Update} {next : SearchState σ nfa} {update : σ.Update} {state : Fin nfa.size} {stack' : εStack σ nfa}
+variable {s : String} {α : Type} {tracker : PosTracker s α} {nfa : NFA} {wf : nfa.WellFormed} {pos : Pos s}
+  {matched : Option α} {next : SearchState α nfa} {update : α} {state : Fin nfa.size} {stack' : εStack α nfa}
 
-theorem base : εClosure σ nfa wf pos matched next [] = (matched, next) := by
+theorem base : εClosure tracker nfa wf pos matched next [] = (matched, next) := by
   simp [εClosure]
 
 theorem visited (hmem : state ∈ next.states) :
-  εClosure σ nfa wf pos matched next ((update, state) :: stack') = εClosure σ nfa wf pos matched next stack' := by
+  εClosure tracker nfa wf pos matched next ((update, state) :: stack') = εClosure tracker nfa wf pos matched next stack' := by
   grind [εClosure]
 
 theorem not_visited (hmem : state ∉ next.states) :
@@ -153,8 +154,8 @@ theorem not_visited (hmem : state ∉ next.states) :
   letI matched' := if node = Node.done then matched <|> some update else matched
   letI states' := next.states.insert state hmem
   letI updates' := if writeUpdate node = true then next.updates.set state update else next.updates
-  εClosure σ nfa wf pos matched next ((update, state) :: stack') =
-  εClosure σ nfa wf pos matched' ⟨states', updates'⟩ (pushNext σ nfa pos node (wf.inBounds state state.isLt) update stack') := by
+  εClosure tracker nfa wf pos matched next ((update, state) :: stack') =
+  εClosure tracker nfa wf pos matched' ⟨states', updates'⟩ (pushNext tracker nfa pos node (wf.inBounds state state.isLt) update stack') := by
   grind [εClosure]
 
 end
