correctness/RegexCorrectness/VM/Search/Basic.lean
@@ -3,6 +3,7 @@ module
 import all RegexCorrectness.VM.Path
 import all RegexCorrectness.VM.EpsilonClosure
 import all RegexCorrectness.VM.CharStep
+import Regex.Strategy
 
 open Regex.Data (SparseSet)
 open Regex (NFA)
@@ -12,8 +13,8 @@ namespace Regex.VM
 
 variable {s : String}
 
-theorem captureNext.go.induct' (σ : Strategy s) (nfa : NFA) (wf : nfa.WellFormed)
-  (motive : Pos s → Option σ.Update → SearchState σ nfa → SearchState σ nfa → Prop)
+theorem captureNext.go.induct' {α : Type} (tracker : PosTracker s α) (nfa : NFA) (wf : nfa.WellFormed)
+  (motive : Pos s → Option α → SearchState α nfa → SearchState α nfa → Prop)
   (not_found : ∀ matched current next,
     motive s.endPos matched current next)
   (found : ∀ pos matched current next,
@@ -22,62 +23,62 @@ theorem captureNext.go.induct' (σ : Strategy s) (nfa : NFA) (wf : nfa.WellForme
     matched.isSome →
     motive pos matched current next)
   (ind_not_found : ∀ pos matched current next ne,
-    let stepped := eachStepChar σ nfa wf pos ne current next
-    let expanded := εClosure σ nfa wf (pos.next ne) .none stepped.2 [(σ.empty, ⟨nfa.start, wf.start_lt⟩)]
+    let stepped := eachStepChar tracker nfa wf pos ne current next
+    let expanded := εClosure tracker nfa wf (pos.next ne) .none stepped.2 [(tracker.empty, ⟨nfa.start, wf.start_lt⟩)]
     matched = .none →
     stepped.1 = .none →
     motive (pos.next ne) expanded.1 expanded.2 ⟨current.states.clear, current.updates⟩ →
     motive pos matched current next)
   (ind_found : ∀ pos matched current next ne,
-    let stepped := eachStepChar σ nfa wf pos ne current next
+    let stepped := eachStepChar tracker nfa wf pos ne current next
     (matched.isSome → ¬current.states.isEmpty) →
     matched.isSome ∨ stepped.1.isSome →
     motive (pos.next ne) (stepped.1 <|> matched) stepped.2 ⟨current.states.clear, current.updates⟩ →
     motive pos matched current next)
-  (pos : Pos s) (matched : Option σ.Update) (current next : SearchState σ nfa) :
+  (pos : Pos s) (matched : Option α) (current next : SearchState α nfa) :
   motive pos matched current next :=
-  captureNext.go.induct σ nfa wf motive
+  captureNext.go.induct tracker nfa wf motive
     (fun matched current next => not_found matched current next)
     (fun pos matched current next ne h =>
       found pos matched current next ne (by grind) (by grind))
     (fun pos matched current next ne h₁ h₂ ih => by
-      let stepped := eachStepChar σ nfa wf pos ne current next
-      let expanded := εClosure σ nfa wf pos .none stepped.2 [(σ.empty, ⟨nfa.start, wf.start_lt⟩)]
+      let stepped := eachStepChar tracker nfa wf pos ne current next
+      let expanded := εClosure tracker nfa wf (pos.next ne) .none stepped.2 [(tracker.empty, ⟨nfa.start, wf.start_lt⟩)]
       rw [Option.isNone_iff_eq_none, Option.orElse_eq_none] at h₂
       exact ind_not_found pos matched current next ne h₂.2 h₂.1 ih)
     (fun pos matched current next ne h₁ h₂ ih => by
-      let stepped := eachStepChar σ nfa wf pos ne current next
+      let stepped := eachStepChar tracker nfa wf pos ne current next
       exact ind_found pos matched current next ne (by grind) (by grind [Option.isSome_iff_ne_none]) ih)
     pos matched current next
 
 section
 
 @[simp, grind =]
-theorem captureNext.go_not_found {σ nfa wf matched current next} :
-  captureNext.go σ nfa wf s.endPos matched current next = matched := by
+theorem captureNext.go_not_found {α : Type} {tracker : PosTracker s α} {nfa wf matched current next} :
+  captureNext.go tracker nfa wf s.endPos matched current next = matched := by
   grind [captureNext.go]
 
 @[simp, grind =]
-theorem captureNext.go_found {σ nfa wf pos matched current next}
+theorem captureNext.go_found {α : Type} {tracker : PosTracker s α} {nfa wf pos matched current next}
   (ne : pos ≠ s.endPos) (isEmpty : current.states.isEmpty) (isSome : matched.isSome) :
-  captureNext.go σ nfa wf pos matched current next = matched := by
+  captureNext.go tracker nfa wf pos matched current next = matched := by
   grind [captureNext.go]
 
 @[simp, grind =>]
-theorem captureNext.go_ind_not_found {σ : Strategy s} {nfa wf pos matched current next ne} (stepped expanded)
-  (eq₁ : stepped = eachStepChar σ nfa wf pos ne current next)
-  (eq₂ : expanded = εClosure σ nfa wf (pos.next ne) .none stepped.2 [(σ.empty, ⟨nfa.start, wf.start_lt⟩)])
+theorem captureNext.go_ind_not_found {α : Type} {tracker : PosTracker s α} {nfa wf pos matched current next ne} (stepped expanded)
+  (eq₁ : stepped = eachStepChar tracker nfa wf pos ne current next)
+  (eq₂ : expanded = εClosure tracker nfa wf (pos.next ne) .none stepped.2 [(tracker.empty, ⟨nfa.start, wf.start_lt⟩)])
   (isNone₁ : matched = .none) (isNone₂ : stepped.1 = .none) :
-  captureNext.go σ nfa wf pos matched current next =
-  captureNext.go σ nfa wf (pos.next ne) expanded.1 expanded.2 ⟨current.states.clear, current.updates⟩ := by
+  captureNext.go tracker nfa wf pos matched current next =
+  captureNext.go tracker nfa wf (pos.next ne) expanded.1 expanded.2 ⟨current.states.clear, current.updates⟩ := by
   grind [captureNext.go]
 
 @[simp, grind →]
-theorem captureNext.go_ind_found {σ : Strategy s} {nfa wf pos matched current next ne} (stepped)
-  (eq : stepped = eachStepChar σ nfa wf pos ne current next)
+theorem captureNext.go_ind_found {α : Type} {tracker : PosTracker s α} {nfa wf pos matched current next ne} (stepped)
+  (eq : stepped = eachStepChar tracker nfa wf pos ne current next)
   (hemp : matched.isSome → ¬current.states.isEmpty) (isSome : matched.isSome ∨ stepped.1.isSome) :
-  captureNext.go σ nfa wf pos matched current next =
-  captureNext.go σ nfa wf (pos.next ne) (stepped.1 <|> matched) stepped.2 ⟨current.states.clear, current.updates⟩ := by
+  captureNext.go tracker nfa wf pos matched current next =
+  captureNext.go tracker nfa wf (pos.next ne) (stepped.1 <|> matched) stepped.2 ⟨current.states.clear, current.updates⟩ := by
   grind [captureNext.go, Option.orElse_eq_orElse, Option.isNone_iff_eq_none]
 
 end
